link: almost updated, few ghost updates need to be added

link.v
@@ -66,6 +66,8 @@ Section Link_Template.
    * assumed by the template. See GRASShopper files b-link-core.spl and
    * hashtbl-link.spl for the concrete implementations. *)
 
+  (* TODO add alias inreach = inset for this file. *)
+
   Parameter findNext : val.
   Parameter decisiveOp : (dOp → val).
 
@@ -77,9 +79,9 @@ Section Link_Template.
       | SOME "n'" => unlockNode "n";; "tr" "n'" "k"
       end.
 
-  Definition CSSOp (Ψ: dOp) (root: Node) : val :=
+  Definition CSSOp (Ψ: dOp) (r: Node) : val :=
     rec: "dictOp" "k" :=
-      let: "n" := traverse #root "k" in
+      let: "n" := traverse #r "k" in
       match: ((decisiveOp Ψ) "n" "k") with
         NONE => unlockNode "n";; "dictOp" "k"
       | SOME "res" => unlockNode "n";; "res"
@@ -133,361 +135,489 @@ Section Link_Template.
   Definition inFP γ_f n : iProp :=
     ∃ (N: gset Node), own γ_f (◯ N) ∗ ⌜n ∈ N⌝.
 
-  Definition nodePred γ_h γ_k n I_n C_n : iProp :=
-    node n I_n C_n ∗ own (γ_h n) ((●{1/2} I_n))
-      ∗ own γ_k (◯ prod (keyset K I_n n, C_n)) ∗ ⌜domm I_n = {[n]}⌝.
+  Definition inInr γ_i k (n: Node) : iProp :=
+    ∃ (Ks: gset K), own (γ_i n) (◯ Ks) ∗ ⌜k ∈ Ks⌝.
 
-  Definition CSS γ_I γ_f γ_k γ_i γ_h root C : iProp :=
-    (∃ I, own γ_I (● I) ∗ ⌜globalinv K root I⌝
-        ∗ own γ_k (● prod (KS, C))
-        ∗ own γ_f (● domm I)
-        ∗ ([∗ set] n ∈ (domm I), (∃ (b: bool) (I_n: inset_flowint_ur K),
-            (lockLoc n) ↦ #b
-            ∗ (if b then True
-               else (∃ C_n, nodePred γ_h γ_k n I_n C_n))
-            ∗ own γ_I (◯ I_n)
-            ∗ own (γ_h n) ((●{1/2} I_n))
-            ∗ ⌜domm I_n = {[n]}⌝ (* TODO Can this be removed? *)
-            ∗ own (γ_i n) (● (inset K I_n n))))
+  Definition nodePred γ_f γ_h γ_k n In Cn : iProp :=
+    node n In Cn
+    ∗ own (γ_h n) ((●{1/2} In))
+    ∗ own γ_k (◯ prod (keyset K In n, Cn))
+    ∗ inFP γ_f n
+    ∗ ⌜domm In = {[n]}⌝.
+
+  Definition nodeShared γ_I γ_i γ_h n In : iProp :=
+    own γ_I (◯ In)
+    ∗ own (γ_h n) ((●{1/2} In))
+    ∗ ⌜domm In = {[n]}⌝    (* Needed for globalinv_root_ins *)
+    ∗ own (γ_i n) (● (inset K In n)).
+
+  Definition CSSi γ_I γ_f γ_k γ_i γ_h r C I : iProp :=
+    (own γ_I (● I) ∗ ⌜globalinv K r I⌝
+     ∗ own γ_k (● prod (KS, C))
+     ∗ own γ_f (● domm I)
+     ∗ ([∗ set] n ∈ (domm I), (∃ (b: bool) (In: inset_flowint_ur K),
+         (lockLoc n) ↦ #b
+         ∗ (if b then True else (∃ Cn, nodePred γ_f γ_h γ_k n In Cn))
+         ∗ nodeShared γ_I γ_i γ_h n In))
     )%I.
 
+  Definition CSS γ_I γ_f γ_k γ_i γ_h r C : iProp :=
+    (∃ I, CSSi γ_I γ_f γ_k γ_i γ_h r C I)%I.
+
   (** Some useful lemmas *)
-  
-  Lemma CSS_unfold γ_I γ_f γ_k γ_i γ_h root C n :
-    inFP γ_f n ∗ CSS γ_I γ_f γ_k γ_i γ_h root C
-    -∗ (∃ (I_n: inset_flowint_ur K),
-          (∃ (b: bool), lockLoc n ↦ #b
-          ∗ (if b then True else (∃ C_n, nodePred γ_h γ_k n I_n C_n)))
-        ∗ ((∃ (b: bool), lockLoc n ↦ #b
-             ∗ (if b then True else (∃ C_n, nodePred γ_h γ_k n I_n C_n)))
-           -∗ CSS γ_I γ_f γ_k γ_i γ_h root C)).
+
+  Lemma inFP_domm γ_I γ_f γ_k γ_i γ_h r C I n :
+    inFP γ_f n -∗ CSSi γ_I γ_f γ_k γ_i γ_h r C I -∗ ⌜n ∈ domm I⌝.
   Proof.
-    iIntros "(#Hfp & Hcss)".
-    iDestruct "Hcss" as (I) "(HI & Hglob & Hks & Hdom & Hbigstar)".
+    iIntros "#Hfp Hcss".
+    iDestruct "Hcss" as "(HI & Hglob & Hks & Hdom & Hbigstar)".
     iDestruct "Hfp" as (N) "(#Hdom' & n_in_N)". iDestruct "n_in_N" as %n_in_N.
     iPoseProof ((auth_own_incl γ_f (domm I) N) with "[$]") as "#N_incl".
     iDestruct "N_incl" as %N_incl.
     apply gset_included in N_incl.
-    assert (n ∈ domm I) as n_in_I by set_solver.
+    iPureIntro. set_solver.
+  Qed.
+  
+  Lemma frac_int_equal (γ_h: Node → gname) n In In' :
+    own (γ_h n) (●{1/2} In) -∗ own (γ_h n) (●{1/2} In') -∗ ⌜In = In'⌝.
+  Proof.
+    iIntros.
+    iPoseProof ((own_valid_2 (γ_h n) (●{1/2} In) (●{1/2} In'))
+                  with "[$] [$]") as "%"; try done.
+    iPureIntro.
+    apply (auth_auth_frac_op_inv _ _ _ _) in H0.
+    by apply leibniz_equiv.
+  Qed.
+    
+  Lemma CSS_unfold γ_I γ_f γ_k γ_i γ_h r C n :
+    let globalGhost γ_I γ_k γ_f r I C : iProp :=
+        (own γ_I (● I) ∗ ⌜globalinv K r I⌝ ∗ own γ_k (● prod (KS, C))
+        ∗ own γ_f (● domm I))%I
+    in
+    CSS γ_I γ_f γ_k γ_i γ_h r C -∗ inFP γ_f n
+    -∗ (∃ I,
+        globalGhost γ_I γ_k γ_f r I C
+        ∗ (∃ (b: bool) (In: inset_flowint_ur K),
+              lockLoc n ↦ #b
+              ∗ (if b then True else (∃ Cn, nodePred γ_f γ_h γ_k n In Cn))
+              ∗ nodeShared γ_I γ_i γ_h n In)
+        ∗ (∀ C',
+           (globalGhost γ_I γ_k γ_f r I C'
+           ∗ (∃ (b: bool) (In: inset_flowint_ur K),
+                 lockLoc n ↦ #b
+                 ∗ (if b then True else (∃ Cn, nodePred γ_f γ_h γ_k n In Cn))
+                 ∗ nodeShared γ_I γ_i γ_h n In))
+            -∗ CSS γ_I γ_f γ_k γ_i γ_h r C')).
+  Proof.
+    iIntros "Hcss #Hfp".
+    iDestruct "Hcss" as (I) "(HI & Hglob & Hks & Hdom & Hbigstar)".
+    iPoseProof (inFP_domm with "[$] [$]") as "%".
     rewrite (big_sepS_elem_of_acc _ (domm I) n); last by eauto.
-    iDestruct "Hbigstar" as "(Hn & Hbigstar)".
-    iDestruct "Hn" as (b In) "(Hlock & Hb & HIn & HhIn & HdomIn & Hins)".
-    iExists In. iSplitL "Hlock Hb".
-    - iExists b. by iFrame "∗".
-    - iIntros "Hn".  clear b. iDestruct "Hn" as (b) "(Hn & Hite)". 
-      iExists I. iFrame "∗". iApply "Hbigstar".
-      iExists b, In. auto with iFrame. 
+    iDestruct "Hbigstar" as "(Hn & Hbigstar)". iExists I. iFrame "∗".
+    iIntros (C') "((HI & Hglob & Hks & Hdom) & H)".
+    iExists I. iFrame "∗". by iApply "Hbigstar".
   Qed.
 
-  Lemma CSS_fold γ_I γ_f γ_k γ_i γ_h root C n I_n C_n :
-    nodePred γ_h γ_k n I_n C_n ∗ CSS γ_I γ_f γ_k γ_i γ_h root C
-    -∗ (lockLoc n ↦ #true ∗ nodePred γ_h γ_k n I_n C_n
-        ∗ ((∃ (b: bool), lockLoc n ↦ #b
-             ∗ (if b then True else (∃ C_n, nodePred γ_h γ_k n I_n C_n)))
-           -∗ CSS γ_I γ_f γ_k γ_i γ_h root C)).
+  Lemma CSS_unfold_node γ_I γ_f γ_k γ_i γ_h r C n In Cn :
+    let globalGhost γ_I γ_k γ_f r I C : iProp :=
+        (own γ_I (● I) ∗ ⌜globalinv K r I⌝ ∗ own γ_k (● prod (KS, C))
+        ∗ own γ_f (● domm I))%I
+    in
+    CSS γ_I γ_f γ_k γ_i γ_h r C -∗ node n In Cn -∗ inFP γ_f n
+    -∗ own (γ_h n) (●{1/2} In)
+    -∗ (∃ I,
+        node n In Cn ∗ own (γ_h n) (●{1/2} In)
+        ∗ globalGhost γ_I γ_k γ_f r I C
+        ∗ lockLoc n ↦ #true ∗ nodeShared γ_I γ_i γ_h n In
+        ∗ (∀ C',
+           (globalGhost γ_I γ_k γ_f r I C'
+           ∗ (∃ (b: bool) (In: inset_flowint_ur K),
+                 lockLoc n ↦ #b
+                 ∗ (if b then True else (∃ Cn, nodePred γ_f γ_h γ_k n In Cn))
+                 ∗ nodeShared γ_I γ_i γ_h n In))
+            -∗ CSS γ_I γ_f γ_k γ_i γ_h r C')).
   Proof.
-    iIntros "(Hn & Hcss)".
+    iIntros "Hcss Hn #Hfp HfIn".
+    iPoseProof (CSS_unfold with "[$] [$]") as (I) "(Hg & Hns & Hcss')".
+    iExists I.
+    iDestruct "Hns" as (b In') "(Hlock & Hnp & Hns)". destruct b.
+    - (* Case n locked *)
+      iDestruct "Hg" as "(HI & Hglob & Hks & Hdom)".
+      iDestruct "Hns" as "(HIn & HhIn' & HdomIn & Hins)".
+      iPoseProof (frac_int_equal with "[$] [$]") as "%". subst In'.
+      iFrame "∗".
+    - (* Case n unlocked: impossible *)
+      iDestruct "Hnp" as (?C) "(Hn' & _)".
+      iExFalso. iApply (node_sep_star n In In' with "[$]").
+  Qed.
+
+  (* TODO try just using CSS_unfold instead: *)
+  Lemma CSS_fold γ_I γ_f γ_k γ_i γ_h r C n In Cn :
+    nodePred γ_f γ_h γ_k n In Cn -∗ CSS γ_I γ_f γ_k γ_i γ_h r C
+    -∗ (lockLoc n ↦ #true ∗ nodePred γ_f γ_h γ_k n In Cn
+        ∗ ((∃ (b: bool), lockLoc n ↦ #b
+             ∗ (if b then True else (∃ Cn, nodePred γ_f γ_h γ_k n In Cn)))
+           -∗ CSS γ_I γ_f γ_k γ_i γ_h r C)).
+  Proof.
+    iIntros "Hnp Hcss".
     iDestruct "Hcss" as (I) "(HI & Hglob & Hks & Hdom & Hbigstar)".
-    iDestruct "Hn" as "(Hnode & ? & ? & domIn)".
-    iDestruct "domIn" as %domIn.
-    (* TODO CONTINUE: either thread inFP through the proof or put the frac singleton interface inside nodePred *)
-    iPoseProof ((auth_own_incl γ_I (I) (I_n)) with "[$]") as "%".
-    rename H0 into I_incl. destruct I_incl as [Io I_incl].
-    iPoseProof (own_valid with "H●I") as "%". rename H0 into Valid_I.
-    assert (n ∈ domm I) as n_in_I.
-    { rewrite I_incl. rewrite flowint_comp_fp.
-      rewrite domIn. set_solver. rewrite <- I_incl.
-      by apply auth_auth_valid. } 
+    iDestruct "Hnp" as "(Hn & HnhIn & HkIn & #Hinfp & domIn)".
+    iPoseProof (inFP_domm with "[$] [$]") as "%".
     rewrite (big_sepS_elem_of_acc _ (domm I) n); last by eauto.
-    iDestruct "Hbigstar" as "(Hn & Hbigstar)".
-    iDestruct "Hn" as (b In) "(Hlock & Hb)".
-    iEval (rewrite <-Hloc).
-    wp_store. iMod ("Hclose" with "[Hnode H◯k H◯I H●I Hglob H●k H●f Hlock Hb Hbigstar]") as "HΦ".
-    iExists I. iFrame "∗". iApply "Hbigstar".
-    iExists false, I_n. iFrame. destruct b.
-    iExists C_n. iFrame "∗ %". iDestruct "Hb" as (Cn') "Hn'".
-    unfold nodePred.
-    iDestruct "Hn'" as "(Hnode' & _)". 
-    iExFalso. iApply node_sep_star. iFrame. 
-    iModIntro. done.
+    iDestruct "Hbigstar" as "(Hns & Hbigstar)".
+    iDestruct "Hns" as (b In') "(Hlock & Hb & HIn & HhIn & HdomIn & Hins)".
+    destruct b; first last.
+    - (* Case n unlocked: impossible *)
+      iDestruct "Hb" as (?C) "(Hn' & _)".
+      iExFalso. iApply (node_sep_star n In In' with "[$]").
+    - (* Case n locked *)
+      iPoseProof (frac_int_equal with "[$] [$]") as "%". subst In'.
+      iFrame "Hlock Hn HnhIn HkIn Hinfp domIn".
+      iIntros "H". iClear "Hb". iDestruct "H" as (b) "(Hlock & Hb)".
+      iExists I. iFrame "∗". iApply "Hbigstar".
+      iExists b, In. iFrame "∗". 
+  Qed.
 
+  Lemma inInr_impl_inset γ_I γ_f γ_k γ_i γ_h r C n In Cn k :
+    CSS γ_I γ_f γ_k γ_i γ_h r C -∗ nodePred γ_f γ_h γ_k n In Cn
+    -∗ inInr γ_i k n
+    -∗ ⌜in_inset K k In n⌝.
+  Proof.
+    iIntros "Hcss Hnp Hinr".
+    iDestruct "Hnp" as "(Hn & HnhIn & HkIn & #Hinfp & domIn)".
+    iPoseProof (CSS_unfold_node with "[$] [$] [$] [$]")
+      as (I) "(Hn & HhIn & Hg & Hlock & Hns & Hcss')".
+    iDestruct "Hg" as "(HI & Hglob & Hks & Hdom)".
+    iDestruct "Hns" as "(HIn & HhIn' & HdomIn & Hins)".
+    iDestruct "Hinr" as (R) "(Hinr & %)".
+    iPoseProof ((auth_own_incl (γ_i n) (inset K In n) R) with "[$]")
+      as "incl".
+    iDestruct "incl" as %incl. iPureIntro.
+    apply gset_included in incl. set_solver.
+  Qed.
 
-  Admitted.
+  Lemma ghost_snapshot_fp γ_f (Ns: gset Node) n:
+    ⊢ own γ_f (● Ns) -∗ ⌜n ∈ Ns⌝ ==∗ own γ_f (● Ns) ∗ inFP γ_f n.
+  Proof.
+    iIntros. 
+    iMod (own_update γ_f (● Ns) (● Ns ⋅ ◯ Ns) with "[$]")
+      as "H".
+    { apply auth_update_core_id. apply gset_core_id. done. }
+    iDestruct "H" as "(Haa & Haf)". iFrame. iModIntro.
+    iExists Ns. by iFrame.
+  Qed.
     
+  Lemma ghost_update_step γ_I γ_f γ_k γ_i γ_h r C n In Cn k n' :
+    ⊢ CSS γ_I γ_f γ_k γ_i γ_h r C
+      -∗ nodePred γ_f γ_h γ_k n In Cn
+      -∗ ⌜in_inset K k In n⌝
+      -∗ ⌜in_outset K k In n'⌝
+      ==∗ CSS γ_I γ_f γ_k γ_i γ_h r C ∗ nodePred γ_f γ_h γ_k n In Cn
+      ∗ inFP γ_f n' ∗ inInr γ_i k n'.
+  Proof.
+    iIntros "Hcss Hnp % %".
+    iDestruct "Hnp" as "(Hn & HnhIn & HkIn & #Hinfp & domIn)".
+    (* Can't use CSS_unfold_node because need to unroll bigstar twice. *)
+    iDestruct "Hcss" as (I) "Hcss".
+    iPoseProof (inFP_domm with "[$] [$]") as "%".
+    iDestruct "Hcss" as "(HI & % & Hks & Hdom & Hbigstar)".
+    rewrite (big_sepS_elem_of_acc _ (domm I) n); last by eauto.
+    iDestruct "Hbigstar" as "(Hns & Hbigstar)".
+    
+    iDestruct "Hns" as "(HIn & HhIn' & HdomIn & Hins)".
+    (* In ≼ I *)
+    iPoseProof ((auth_own_incl γ_I I In) with "[$]")
+      as (Io) "incl".
+    iDestruct "incl" as %incl.
+    assert (n' ∈ domm Io).
+      by eauto using flowint_step. 
+    assert (n' ∈ domm I).
+      by admit.
+    (* Take snapshot of fp to get inFP n' *)
+    iMod (ghost_snapshot_fp γ_f (domm I) n' with "[$Hdom] [% //]")
+        as "(Hdom & #Hinfp')".
+
+      
+    (* unroll star again using n' ∈ domm (I - In) and get In' *)
+    (* somehow get ✓ (In ⋅ In') *)
+    (* flowint_inset_step gives me k ∈ inset In' *)
+    (* snapshot In' inreach to get inInr k n' *)
+  Admitted.
+
+  Lemma ghost_update_root γ_I γ_f γ_k γ_i γ_h r C k :
+    ⊢ CSS γ_I γ_f γ_k γ_i γ_h r C -∗ ⌜k ∈ KS⌝
+      ==∗
+      CSS γ_I γ_f γ_k γ_i γ_h r C ∗ inFP γ_f r ∗ inInr γ_i k r.
+  Proof.
+    iIntros "Hcss %".
+    iDestruct "Hcss" as (I) "(HI & #Hglob & Hks & Hdom & Hbigstar)".
+    iDestruct "Hglob" as %Hglob.
+    (* Snapshot FP for inFP: *)
+    iMod (own_update γ_f (● domm I) (● domm I ⋅ ◯ domm I) with "Hdom")
+      as "(Hdom & #Hfp)".
+    { apply auth_update_core_id. apply gset_core_id. done. }
+    (* Unfold bigstar *)
+    assert (r ∈ domm I)%I as Hroot.
+    { apply globalinv_root_fp. done. }
+    rewrite (big_sepS_elem_of_acc _ (domm I) r); last by eauto.
+    iDestruct "Hbigstar" as "[Hn Hbigstar]".
+    iDestruct "Hn" as (b Ir) "(H1 & H2 & H3 & H4 & % & Hksr)". (* TODO rename *)
+    (* Get Ir ≼ I needed for globalinv_root_ins *)
+    iPoseProof (auth_own_incl with "[$HI $H3]") as "%".
+    iAssert (inFP γ_f r)%I as "#Hinfp".
+    {
+      unfold inFP. iExists (domm I). iFrame "Hfp".
+      iPureIntro. by apply globalinv_root_fp.
+    }
+    iMod (own_update (γ_i r) _ (● (inset K Ir r) ⋅ ◯ (inset K Ir r))
+            with "Hksr") as "(Hksr & #Hinr)".
+    { apply auth_update_core_id. apply gset_core_id. done. }
+    (* Hksr -> Hinr *)
+    iAssert (inInr γ_i k r)%I as "#Hininr".
+    {
+      iExists (inset K Ir r). iFrame "Hinr". iPureIntro.
+      apply (globalinv_root_ins I). done. 
+    }
+    iModIntro. iSplitL. iExists I. iFrame "∗". iSplitR; first by iPureIntro.
+    iApply "Hbigstar". iExists b, Ir. iFrame "∗". by iPureIntro.
+    iFrame "#".
+  Qed.
+
+  Lemma ghost_update_CSS γ_I γ_f γ_k γ_i γ_h r C n In Cn Cn' (k: K) :
+    ⊢ CSS γ_I γ_f γ_k γ_i γ_h r C -∗ ⌜k ∈ KS⌝
+      -∗ node n In Cn'
+      -∗ own (γ_h n) (●{1/2} In) -∗ own γ_k (◯ prod (keyset K In n, Cn))
+      ==∗ ∃ C', CSS γ_I γ_f γ_k γ_i γ_h r C' ∗ nodePred γ_f γ_h γ_k n In Cn'.
+  Proof.
+(* Proof of ghost_update_CSS: *)
+      (* iAssert (⌜n ∈ domm I⌝)%I with "[Hdom]" as "%". *)
+      (* { iPoseProof ((auth_own_incl γ_f (domm I) Ns) with "[$]") as "%". *)
+      (*   apply gset_included in H1. *)
+      (* iPureIntro. set_solver. } *)
+      (* rewrite (big_sepS_elem_of_acc _ (domm I) n); last by eauto. *)
+      (* iDestruct "Hbigstar" as "[Hn Hbigstar]". *)
+      (* iDestruct "Hn" as (b In1) "(Hlock & Hb & HIn & #HNds & Hfis & Hinreach)". *)
+      (* destruct b; first last. { iDestruct "Hb" as (Cn'') "(Hn' & _)". *)
+      (* iAssert (⌜False⌝)%I with "[Hn Hn']" as %Hf. { iApply (node_sep_star n In In1). *)
+      (* iFrame. } exfalso. done. } *)
+      (* iAaccIntro with "Hlock". { iIntros "Hlock". iModIntro. iSplitR "Hfil Hn Hks". *)
+      (* iExists I. iFrame "∗ % #". iApply "Hbigstar". iExists true, In1. *)
+      (* iFrame "∗ # %". eauto with iFrame. } iIntros "Hlock". *)
+      (* iPoseProof (auth_own_incl with "[$HI $HIn]") as (I2)"%". *)
+      (* iPoseProof ((own_valid γ_I (● I)) with "HI") as "%". *)
+      (* iPoseProof ((own_valid_2 (γ_h n) (●{1/2} In) (●{1/2} In1)) with "[Hfil] [Hfis]") as "%"; try done. *)
+      (* apply (auth_auth_frac_op_inv _ _ _ _) in H4. apply leibniz_equiv in H4. replace In1. *)
+      (* iPoseProof ((own_valid γ_I (◯ In)) with "HIn") as "%". rename H5 into HInV. *)
+      (* assert (✓ In) as HInv. { apply (auth_frag_valid (◯ In)). done. }     *)
+      (* iPoseProof (own_valid with "Hks") as "%". rename H5 into HvldCn. *)
+      (* rewrite auth_frag_valid in HvldCn *; intros HvldCn. unfold valid, cmra_valid in HvldCn. *)
+      (* simpl in HvldCn. unfold ucmra_valid in HvldCn. simpl in HvldCn. *)
+      (* iMod ((ghost_update_keyset γ_k dop k Cn Cn' res (keyset K In n) C) with "[HKS Hks]") as "Hgks". *)
+      (* assert (k ∈ keyset K In n). apply keyset_def; try done. iFrame "% ∗ #". *)
+      (* iEval (unfold Ψ) in "HΨ". *)
+      (* { destruct dop. *)
+      (*   - iDestruct "HΨ" as %(HΨ & _). iPureIntro. subst Cn'. done. *)
+      (*   - iDestruct "HΨ" as %(HΨ & _). iPureIntro. set_solver. *)
+      (*   - iDestruct "HΨ" as %(HΨ & _). iPureIntro. set_solver. } *)
+      (* iDestruct "Hgks" as (C') "(#HΨC & Ha & Hf)". *)
+  Admitted.
 
   (** High-level lock specs *)
 
-  Lemma lockNode_spec_high γ_I γ_f γ_k γ_i γ_h root n :
+  Lemma lockNode_spec_high γ_I γ_f γ_k γ_i γ_h r n :
     ⊢ inFP γ_f n
-      -∗ <<< ∀ C, CSS γ_I γ_f γ_k γ_i γ_h root C >>>
+      -∗ <<< ∀ C, CSS γ_I γ_f γ_k γ_i γ_h r C >>>
            lockNode #n @ ⊤
-         <<< ∃ I_n C_n, CSS γ_I γ_f γ_k γ_i γ_h root C
-                      ∗ nodePred γ_h γ_k n I_n C_n,
+         <<< ∃ In Cn, CSS γ_I γ_f γ_k γ_i γ_h r C
+                      ∗ nodePred γ_f γ_h γ_k n In Cn,
              RET #() >>>.
   Proof.
     iIntros "#HFp". iIntros (Φ) "AU".
     awp_apply (lockNode_spec n).
     iApply (aacc_aupd_commit with "AU"); first done.
-    iIntros (C) "HCSS".
-    iPoseProof (CSS_unfold with "[$HFp $HCSS]") as (In) "(Hn & HCSS')".
-    iDestruct "Hn" as (b) "(Hlock & Hn)".
+    iIntros (C) "Hcss".
+    iPoseProof (CSS_unfold with "[$] [$]")
+      as (I) "(Hg & Hn & Hcss')".
+    iDestruct "Hn" as (b In) "(Hlock & Hnp & Hother)".
     iAaccIntro with "Hlock".
     { iIntros "Hlockn". iModIntro.
-      iPoseProof ("HCSS'" with "[Hlockn Hn]") as "HCSS"; first eauto with iFrame.
-      iFrame "HCSS". iIntros "AU". by iModIntro.
+      iPoseProof ("Hcss'" with "[-]") as "Hcss"; first eauto with iFrame.
+      iFrame "Hcss". iIntros "AU". by iModIntro.
     }
     iIntros "(Hlockn & %)". iModIntro.
-    subst b. iDestruct "Hn" as (Cn) "Hn".
-    iPoseProof ("HCSS'" with "[Hlockn]") as "HCSS"; first eauto with iFrame.
-    iExists In, Cn. 
-    iFrame "∗". iIntros "H". by iModIntro.
+    subst b. iDestruct "Hnp" as (Cn) "Hn".
+    iPoseProof ("Hcss'" with "[-Hn]") as "Hcss"; first eauto with iFrame.
+    iExists In, Cn. iFrame "∗". iIntros "H". by iModIntro.
   Qed.
   
-  Lemma unlockNode_spec_high γ_I γ_f γ_k γ_i γ_h root n I_n C_n :
-    ⊢ nodePred γ_h γ_k n I_n C_n
-      -∗ <<< ∀ C, CSS γ_I γ_f γ_k γ_i γ_h root C >>>
+  Lemma unlockNode_spec_high γ_I γ_f γ_k γ_i γ_h r n In Cn :
+    ⊢ nodePred γ_f γ_h γ_k n In Cn
+      -∗ <<< ∀ C, CSS γ_I γ_f γ_k γ_i γ_h r C >>>
            unlockNode #n @ ⊤
-         <<< CSS γ_I γ_f γ_k γ_i γ_h root C, RET #() >>>.
+         <<< CSS γ_I γ_f γ_k γ_i γ_h r C, RET #() >>>.
   Proof.
     iIntros "Hn". iIntros (Φ) "AU".
     awp_apply (unlockNode_spec n).
     iApply (aacc_aupd_commit with "AU"); first done.
-    iIntros (C) "HCSS".
-    iPoseProof (CSS_fold with "[$Hn $HCSS]") as "(Hlock & Hn & HCSS')".
+    iIntros (C) "Hcss".
+    iPoseProof (CSS_fold with "[$Hn] [$Hcss]") as "(Hlock & Hn & Hcss')".
     iAaccIntro with "Hlock".
     { iIntros "Hlock". iModIntro.
-      iPoseProof ("HCSS'" with "[Hlock]") as "HCSS"; first eauto with iFrame.
-      iFrame "HCSS". iIntros "AU". iModIntro. by iFrame. 
+      iPoseProof ("Hcss'" with "[Hlock]") as "Hcss"; first eauto with iFrame.
+      iFrame "Hcss". iIntros "AU". iModIntro. by iFrame. 
     }
     iIntros "Hlock". iModIntro.
-    iPoseProof ("HCSS'" with "[Hlock Hn]") as "HCSS"; first eauto with iFrame.
+    iPoseProof ("Hcss'" with "[Hlock Hn]") as "Hcss"; first eauto with iFrame.
     iFrame "∗". iIntros "H". by iModIntro.
  Qed.
 
   (** Proofs of traverse and CSSOp *)
 
-  Lemma traverse_spec (γ_I γ_f γ_k: gname) (γ_i γ_h: Node → gname)
-      (root: Node) (k: K) (n: Node) (Ns: gset Node) (I_n:inset_flowint_ur K):
-    ⊢ ⌜k ∈ KS⌝ ∗ ⌜n ∈ Ns⌝ ∗ own γ_f (◯ Ns)
-      ∗ own (γ_i n) (◯ (inset K I_n n))
-      ∗ ⌜k ∈ inset K I_n n⌝ -∗
-        <<< ∀ C, CSS γ_I γ_f γ_k γ_i γ_h root C >>>
+  Lemma traverse_spec γ_I γ_f γ_k γ_i γ_h (r: Node) (k: K) (n: Node) :
+    ⊢ ⌜k ∈ KS⌝ -∗ inFP γ_f n -∗ inInr γ_i k n -∗
+        <<< ∀ C, CSS γ_I γ_f γ_k γ_i γ_h r C >>>
             traverse #n #k @ ⊤
-        <<< ∃ (n': Node) (Ns': gsetUR Node) (I_n': inset_flowint_ur K) (Cn': gset K),
-            CSS γ_I γ_f γ_k γ_i γ_h root C ∗ ⌜n' ∈ Ns'⌝
-            ∗ own γ_f (◯ Ns') ∗ node n' I_n' Cn' ∗ own (γ_h n') ((●{1/2} I_n'))
-            ∗ own γ_k (◯ prod (keyset K I_n' n', Cn')) ∗ ⌜domm I_n' = {[n']}⌝
-            ∗ ⌜in_inset K k I_n' n'⌝ ∗ ⌜¬in_outsets K k I_n'⌝, RET #n' >>>.
+        <<< ∃ (n': Node) (In': inset_flowint_ur K) (Cn': gset K),
+            CSS γ_I γ_f γ_k γ_i γ_h r C
+            ∗ nodePred γ_f γ_h γ_k n' In' Cn'
+            ∗ ⌜in_inset K k In' n'⌝ ∗ ⌜¬in_outsets K k In'⌝,
+            RET #n'
+        >>>.
   Proof.
-    iLöb as "IH" forall (n Ns I_n). iIntros "(#Hkks & #Hinn & #Hfp & #Hinrfp & #Hkinr)".
-    iDestruct "Hinn" as %Hinn.
+    iLöb as "IH" forall (n). iIntros "% #Hinfp #Hininr".
     iIntros (Φ) "AU". wp_lam. wp_let. wp_bind(lockNode _)%E.
-    awp_apply (lockNode_spec n). iApply (aacc_aupd_abort with "AU"); first done.
-    iIntros (C0) "Hst". iDestruct "Hst" as (I) "(HI & HKS & HNDS & Hglob & Hstar)".
-    iAssert (⌜n ∈ domm I⌝)%I with "[HNDS]" as "%".
-    { iPoseProof ((auth_own_incl γ_f (domm I) Ns) with "[$]") as "%".
-      apply gset_included in H0.
-      iPureIntro. set_solver. }
-    rewrite (big_sepS_elem_of_acc _ (domm I) n); last by eauto.
-    iDestruct "Hstar" as "[Hn Hstar]".
-    iDestruct "Hn" as (b In) "(Hlock & Hb & HIn & #HNds & Hfis & Hks)".
-    iAaccIntro with "Hlock". { iIntros "H". iModIntro. iSplitL. iFrame "∗ % #".
-    iExists I. iFrame "∗ % #". iApply "Hstar". iExists b, In.
-    iFrame "# % ∗". eauto with iFrame. } iIntros "(Hloc & %)".
-    destruct b. { iExFalso. done. } iModIntro. clear H1.
-    iPoseProof ((auth_own_incl (γ_i n) (inset K In n) (inset K I_n n)) with "[$Hks $Hinrfp]") as "%".
-    apply gset_included in H1.
-    iDestruct "Hkinr" as "%".
-    assert (k ∈ inset K In n) as Hkinr; first by set_solver.
-    iPoseProof (own_valid with "HIn") as "%". rename H3 into HInV.
-    assert (✓ In) as HInv. { apply (auth_frag_valid (◯ In)). done. }
-    iSplitR "Hb". iFrame "∗ % #". iExists I. iFrame "∗ % #". iApply "Hstar". iExists true, In.
-    iFrame "# % ∗". iIntros "AU". iModIntro. wp_pures.
-    iDestruct "Hb" as (Cn) "(Hrep & Hfil & Hks)". iDestruct "HNds" as %HNds.
-    wp_bind (findNext _ _)%E. wp_apply ((findNext_spec n k In Cn) with "[Hrep]").
-    iDestruct "Hkks" as "%".
-    iFrame; iPureIntro; split; done. iIntros (b n') "(Hrep & Hb)". destruct b.
-    - wp_pures. awp_apply (unlockNode_spec n).
-      iApply (aacc_aupd_abort with "AU"); first done. iIntros (C1) "Hst".
-      iDestruct "Hst" as (I1) "(HI & HKS & HNDS & Hglob & Hstar)".
-      iAssert (⌜n ∈ domm I1⌝)%I with "[HNDS]" as "%".
-      { iPoseProof ((auth_own_incl γ_f (domm I1) Ns) with "[$]") as "%".
-        apply gset_included in H3.
-        iPureIntro. set_solver. }
-      rewrite (big_sepS_delete _ (domm I1) n); last by eauto. iDestruct "Hstar" as "(Hcln & Hstar)".
-      iDestruct "Hcln" as (b In1) "(Hlock & Hbb & HIn & #HNds1 & Hfis & Hks1)".
-      destruct b; first last. { iDestruct "Hbb" as (Cn') "(Hrep' & _)".
-      iAssert (⌜False⌝)%I with "[Hrep Hrep']" as %Hf. { iApply (node_sep_star n In In1).
-      iFrame. } exfalso. done. }
-      iPoseProof ((own_valid_2 (γ_h n) (●{1 / 2} In) (●{1 / 2} In1)) with "[Hfil] [Hfis]") as "%"; try done.
-      apply (auth_auth_frac_op_inv _ _ _ _) in H4. apply leibniz_equiv in H4. replace In1.
-      iDestruct "Hb" as %Hb. iDestruct "HNds1" as %HNds1. iDestruct "Hglob" as %Hglob.
-      iPoseProof (auth_own_incl with "[$HI $HIn]") as (I2)"%".
-      iPoseProof (own_valid with "HI") as "%". iAssert (⌜n' ∈ domm I1⌝)%I as "%".
-      { iPureIntro. assert (n' ∈ domm I2).
-        { apply (flowint_step I1 In I2 k n' root); try done. }
-        assert (domm I1 = domm In ∪ domm I2).
-        { rewrite H5. apply flowint_comp_fp.
-          rewrite H5 in H6 * => H6.
-          rewrite <-H5.
-          apply auth_auth_valid.
-          rewrite <-H5 in H6. done.
-        }
-        rewrite H8.
-        set_solver. }
-      (* apply Hglob. } *)
-      assert (n ≠ n') as Hneq.
-      { assert (n' ∉ domm In).
-        { apply (outset_distinct In n').
-          split. done.
-          exists k. done. }
-        rewrite HNds1 in H8. set_solver. }
-      rewrite (big_sepS_delete _ (domm I1 ∖ {[n]}) n'); last first.
-      set_solver. iDestruct "Hstar" as "(Hcln' & Hstar)".
-      iDestruct "Hcln'" as (b In') "(Hlock' & Hbb' & HIn' & #HNds' & Hfis' & Hks1')".
-      iPoseProof ((own_op γ_I (◯ In) (◯ In' )) with "[HIn HIn']") as "H"; first by eauto with iFrame.
-      iPoseProof (own_valid with "H") as "%". rewrite -auth_frag_op in H8.
-      assert (✓ (In ⋅ In')). { apply (auth_frag_valid (◯ (In ⋅ In'))). done. }
-      iDestruct "HNds'" as %HNds'.
-      assert (k ∈ inset K In' n').
-      {
-        apply (flowint_inset_step In In' k n'). done. set_solver.
-        unfold in_outset in Hb. done.
-      }
-      assert (root ∈ domm I1). { apply globalinv_root_fp. done. } iDestruct "H" as "(HIn & HIn')".
-      iMod (own_update (γ_i n') _
-                       (● (inset K In' n')
-                          ⋅ ◯ (inset K In' n'))
-              with "Hks1'") as "HNs".
-      apply auth_update_core_id.
-      apply gset_core_id. done. iDestruct "HNs" as "(Hks1' & #Hinr1')".
-      iAaccIntro with "Hlock". { iIntros "Hlock". iModIntro. iSplitR "Hfil Hks Hrep". iFrame "∗ # %".
-      iExists I1. iFrame "∗ % #". rewrite (big_sepS_delete _ (domm I1) n); last by eauto.
-      iSplitR "Hstar Hbb' HIn' Hfis' Hks1' Hlock'". iExists true, In. iFrame "# % ∗".
-      rewrite (big_sepS_delete _ (domm I1 ∖ {[n]}) n'); last first. set_solver. iFrame. iExists b, In'.
-      iFrame "# % ∗".  iIntros "AU". iModIntro. iFrame "# % ∗". } iIntros "Hlock".
-      iMod (own_update γ_f (● domm I1) (● domm I1 ⋅ ◯ domm I1) with "HNDS") as "HNs".
-      apply auth_update_core_id. apply gset_core_id. done. iDestruct "HNs" as "(HAfp & #Hfp1)".
-      iModIntro. iSplitL. iExists I1. iFrame "∗ % #". rewrite (big_sepS_delete _ (domm I1) n); last by eauto.
-      iSplitR "Hstar Hbb' HIn' Hfis' Hks1' Hlock'". iExists false, In. iFrame "# % ∗". iExists Cn. iFrame.
-      rewrite (big_sepS_delete _ (domm I1 ∖ {[n]}) n'); last first. set_solver. iFrame. iExists b, In'.
-      iFrame "# % ∗". iIntros "AU". iModIntro. wp_pures. iSpecialize ("IH" $! n' (domm I1) In').
-      iApply "IH". iFrame "∗ # %". done.
-    - iApply fupd_wp. iMod "AU" as (C) "[Hst [_ Hclose]]". iSpecialize ("Hclose" $! n Ns In Cn).
-      iMod ("Hclose" with "[Hst Hfil Hks Hrep Hb]") as "HΦ". iDestruct "Hb" as %Hnotout.
-      iFrame "∗ # %". iModIntro. wp_pures. done.
+    awp_apply lockNode_spec_high; first done.
+    (* Open AU to get lockNode pre *)
+    iApply (aacc_aupd_abort with "AU"); first done.
+    iIntros (C) "Hcss".
+    iAaccIntro with "Hcss".
+    { iIntros "H". iModIntro. iFrame. iIntros. iModIntro. iFrame. }
+    iIntros (In Cn) "(Hcss & Hnp)". iModIntro.
+    (* Before closing AU, use CSS to get findNext pre *)
+    iPoseProof (inInr_impl_inset with "[$] [$] [$]")
+      as "%".
+    (* Close AU and move on *)
+    iFrame. iIntros "AU". iModIntro.
+    wp_pures.
+    iDestruct "Hnp" as "(Hn & HnhIn & HkIn & _ & %)".
+    wp_bind (findNext _ _)%E. wp_apply ((findNext_spec n k In Cn) with "[$Hn]").
+    { iPureIntro; split; done. }
+    iIntros (b n') "(Hn & Hout)". destruct b.
+    - (* Case: findNext returns Some n' *)
+      wp_pures. wp_bind (unlockNode _).
+      iDestruct "Hout" as %Hout.
+      (* Fold nodePred again *)
+      iAssert (nodePred γ_f γ_h γ_k n In Cn)%I
+        with "[$Hn $HnhIn $HkIn $Hinfp]" as "Hnp"; first by iPureIntro.
+      (* Get traverse's pre before giving up (node n) when calling unlock *)
+      iApply fupd_wp. clear C. iMod "AU" as (C) "[Hcss [Hclose _]]".
+      iMod (ghost_update_step with "[$] [$] [% //] [% //]")
+        as "(Hcss & Hnp & #Hinfp' & #Hininr')".
+      (* Close AU after getting traverse's pre *)
+      iMod ("Hclose" with "Hcss") as "AU". clear C. iModIntro.
+      awp_apply (unlockNode_spec_high with "Hnp").
+      (* Open AU for unlockNode's pre *)
+      iApply (aacc_aupd_abort with "AU"); first done. iIntros (C) "Hcss".
+      iAaccIntro with "Hcss".
+      { iIntros. iModIntro. iFrame. iIntros "AU". iModIntro. iFrame. }
+      (* The last line should really be a tactic.. *)
+      iIntros "Hcss". iModIntro.
+      (* Close up AU again *)
+      iFrame. iIntros "AU". iModIntro. 
+      wp_pures. iSpecialize ("IH" $! n').
+      iApply ("IH" with "[% //] [$] [$]"). done.
+    - (* Case: findNext returns None *)
+      (* Open AU and commit *)
+      iApply fupd_wp. clear C. iMod "AU" as (C) "[Hcss [_ Hclose]]".
+      iSpecialize ("Hclose" $! n In Cn).
+      iAssert (nodePred γ_f γ_h γ_k n In Cn)%I
+        with "[$Hn $HnhIn $HkIn $Hinfp]" as "Hnp"; first by iPureIntro.
+      iMod ("Hclose" with "[$Hcss $Hnp $Hout]") as "HΦ"; first by iPureIntro.
+      iModIntro. wp_pures. done.
   Qed.
 
   (** Verification of abstract specification of the search structure operation. *)
-  
-  Theorem CSSOp_spec (γ_I γ_f γ_k: gname) γ_i γ_h root (k: K) (dop: dOp):
-    ⌜k ∈ KS⌝ -∗ <<< ∀ C, CSS γ_I γ_f γ_k γ_i γ_h root C >>>
-      CSSOp dop root #k @ ⊤
-    <<< ∃ C' (res: bool), CSS γ_I γ_f γ_k γ_i γ_h root C'
+    
+  Theorem CSSOp_spec (γ_I γ_f γ_k: gname) γ_i γ_h r (k: K) (dop: dOp):
+    ⌜k ∈ KS⌝ -∗ <<< ∀ C, CSS γ_I γ_f γ_k γ_i γ_h r C >>>
+      CSSOp dop r #k @ ⊤
+    <<< ∃ C' (res: bool), CSS γ_I γ_f γ_k γ_i γ_h r C'
         ∗ (Ψ dop k C C' res : iProp), RET #res >>>.
   Proof.
-    iIntros "HKin" (Φ) "AU". iLöb as "IH". wp_lam.
-    iApply fupd_wp. iMod "AU" as (C0) "[Hst [HAU _]]".
-    iDestruct "Hst" as (I0) "(HI & HKS & HNDS & #Hglob & Hstar)".
-    iDestruct "Hglob" as %Hglob. iDestruct "HKin" as %HKin.
-    assert (root ∈ domm I0)%I as Hroot. { apply globalinv_root_fp. done. }
-    iMod (own_update γ_f (● domm I0) (● domm I0 ⋅ ◯ domm I0) with "HNDS") as "H".
-    { apply auth_update_core_id. apply gset_core_id. done. }
-    iDestruct "H" as "(HNDS & #Hfp0)".
-    rewrite (big_sepS_elem_of_acc _ (domm I0) root); last by eauto.
-    iDestruct "Hstar" as "[Hn Hstar]".
-    iDestruct "Hn" as (b Ir) "(H1 & H2 & H3 & H4 & H5 & Hksr)".
-    iPoseProof (auth_own_incl with "[$HI $H3]") as "%". iDestruct "H4" as %HNdsr.
-    iMod (own_update (γ_i root) _
-                     (● (inset K Ir root)
-                      ⋅ ◯ (inset K Ir root))
-            with "Hksr") as "H".
-    apply auth_update_core_id. apply gset_core_id. done. iDestruct "H" as "(Hksr & #Hinr)".
-    iMod ("HAU" with "[HI HKS H1 H2 H3 H5 Hstar HNDS Hksr] ") as "AU".
-    { iExists I0. iFrame "∗ % #". iApply "Hstar". iExists b, Ir. iFrame "∗ # %". }
+    iIntros "%" (Φ) "AU". iLöb as "IH". wp_lam.
+    (* Open AU for traverse's pre *)
+    iApply fupd_wp. iMod "AU" as (?) "[Hcss [Hclose _]]".
+    iMod (ghost_update_root with "[$] [% //]") as "(Hcss & ? & ?)".
+    iMod ("Hclose" with "[$] ") as "AU".
     iModIntro. wp_bind (traverse _ _)%E.
-    awp_apply (traverse_spec γ_I γ_f γ_k γ_i γ_h root k root (domm I0) Ir). iFrame "∗ # %".
-    iPureIntro. apply (globalinv_root_ins I0 Ir root k); try done.
+    awp_apply (traverse_spec with "[% //] [$] [$]").
+    (* Open AU for traverse's atomic pre *)
     iApply (aacc_aupd_abort with "AU"); first done.
-    iIntros (C1) "Hst". iAaccIntro with "Hst"; first by eauto with iFrame.
-    iIntros (n Ns In Cn) "(Hst & #Hinn & #Hfp & Hrepn & Hfil & Hks & #HNdsn & #Hinset & #Hnotout)".
-    iDestruct "Hinn" as %Hinn. iDestruct "Hinset" as %Hinset. iDestruct "Hnotout" as %Hnotout.
-    iModIntro. iFrame. iIntros "AU". iModIntro. wp_pures. wp_bind (decisiveOp _ _ _)%E.
-    wp_apply ((decisiveOp_spec dop n k In Cn) with "[Hrepn]"). eauto with iFrame.
-    iIntros (b' res Cn'). iIntros "Hb". destruct b'.
-    - iDestruct "Hb" as "(Hrep & #HΨ)".
+    iIntros (?) "Hcss".
+    iAaccIntro with "Hcss"; first by eauto with iFrame.
+    (* Get traverse's post and close AU *)
+    iIntros (n In Cn) "(Hcss & Hnp & Hinset & Hnotout)".
+    iDestruct "Hinset" as %Hinset. iDestruct "Hnotout" as %Hnotout.
+    iModIntro. iFrame. iIntros "AU". iModIntro.
+    (* Execute decisiveOp *)
+    wp_pures. wp_bind (decisiveOp _ _ _)%E.
+    iDestruct "Hnp" as "(Hn & HnhIn & HkIn & #Hinfp & domIn)".
+    wp_apply (decisiveOp_spec with "[$Hn]"); first by iPureIntro.
+    iIntros (b res Cn'). iIntros "(Hn & Hb)". destruct b.
+    - (* Case: decisiveOp succeeds *)
+      iDestruct "Hb" as "#HΨ".
       wp_pures. wp_bind(unlockNode _)%E.
+      (* Note: cannot use unlockNode_spec_high here because 
+         that needs nodePred, which we won't have until we linearize,
+         which we can't do until we open the AU.
+         We can't open the AU before unlockNode, because linearizing will
+         mean committing the AU and giving up CSS (needed by unlockNode).
+         So we manually execute unlockNode_spec and linearize simultaneously.
+         TODO: would it work if nodePred was inside atomic pre of lockNode?
+       *)
       awp_apply (unlockNode_spec n).
-      iApply (aacc_aupd_commit with "AU"); first done. iIntros (C2) "Hst".
-      iDestruct "Hst" as (I) "(HI & HKS & HNDS & #Hglob & Hstar)".
-      iDestruct "Hglob" as %Hglob'.
-      iAssert (⌜n ∈ domm I⌝)%I with "[HNDS]" as "%".
-      { iPoseProof ((auth_own_incl γ_f (domm I) Ns) with "[$]") as "%".
-        apply gset_included in H1.
-      iPureIntro. set_solver. }
-      rewrite (big_sepS_elem_of_acc _ (domm I) n); last by eauto.
-      iDestruct "Hstar" as "[Hn Hstar]".
-      iDestruct "Hn" as (b' In1) "(Hlock & Hb & HIn & #HNds & Hfis & Hinreach)".
-      destruct b'; first last. { iDestruct "Hb" as (Cn'') "(Hrep' & _)".
-      iAssert (⌜False⌝)%I with "[Hrep Hrep']" as %Hf. { iApply (node_sep_star n In In1).
-      iFrame. } exfalso. done. }
-      iAaccIntro with "Hlock". { iIntros "Hlock". iModIntro. iSplitR "Hfil Hrep Hks".
-      iExists I. iFrame "∗ % #". iApply "Hstar". iExists true, In1.
-      iFrame "∗ # %". eauto with iFrame. } iIntros "Hlock".
-      iPoseProof (auth_own_incl with "[$HI $HIn]") as (I2)"%".
-      iPoseProof ((own_valid γ_I (● I)) with "HI") as "%".
-      iPoseProof ((own_valid_2 (γ_h n) (●{1 / 2} In) (●{1 / 2} In1)) with "[Hfil] [Hfis]") as "%"; try done.
-      apply (auth_auth_frac_op_inv _ _ _ _) in H4. apply leibniz_equiv in H4. replace In1.
-      iPoseProof ((own_valid γ_I (◯ In)) with "HIn") as "%". rename H5 into HInV.
-      assert (✓ In) as HInv. { apply (auth_frag_valid (◯ In)). done. }    
-      iPoseProof (own_valid with "Hks") as "%". rename H5 into HvldCn.
-      rewrite auth_frag_valid in HvldCn *; intros HvldCn. unfold valid, cmra_valid in HvldCn.
-      simpl in HvldCn. unfold ucmra_valid in HvldCn. simpl in HvldCn.
-      iMod ((ghost_update_keyset γ_k dop k Cn Cn' res (keyset K In n) C2) with "[HKS Hks]") as "Hgks".
-      assert (k ∈ keyset K In n). apply keyset_def; try done. iFrame "% ∗ #".
-      iEval (unfold Ψ) in "HΨ".
-      { destruct dop.
-        - iDestruct "HΨ" as %(HΨ & _). iPureIntro. subst Cn'. done.
-        - iDestruct "HΨ" as %(HΨ & _). iPureIntro. set_solver.
-        - iDestruct "HΨ" as %(HΨ & _). iPureIntro. set_solver. }
-      iDestruct "Hgks" as (C2') "(#HΨC & Ha & Hf)".
-      iModIntro. iExists (C2'), res. iSplitL. iSplitR "HΨC".
-      { iExists I. iFrame "∗ % #".
-      iApply "Hstar". iExists false, In.
-      iFrame "∗ % #". iExists Cn'. eauto with iFrame. } done.
-      iIntros "HΦ". iModIntro. wp_pures. done.
-    - wp_match. awp_apply (unlockNode_spec n).
-      iApply (aacc_aupd_abort with "AU"); first done. iIntros (C2) "Hst".
-      iDestruct "Hst" as (I) "(HI & HKS & HNDS & #Hglob & Hstar)".
-      iDestruct "Hglob" as %Hglob'.
-      iAssert (⌜n ∈ domm I⌝)%I with "[HNDS]" as "%".
-      { iPoseProof ((auth_own_incl γ_f (domm I) Ns) with "[$]") as "%".
-        apply gset_included in H1.
-      iPureIntro. set_solver. }
-      rewrite (big_sepS_elem_of_acc _ (domm I) n); last by eauto.
-      iDestruct "Hstar" as "[Hn Hstar]".
-      iDestruct "Hn" as (b' In1) "(Hlock & Hb' & HIn & #HNds & Hfis & Hinreach)".
-      destruct b'; first last.
-      { iDestruct "Hb'" as (Cn'') "(Hrep' & _)".
-        iAssert (⌜False⌝)%I with "[Hb Hrep']" as %Hf.
-        { iDestruct "Hb" as "(Hrep & %)".
-          iApply (node_sep_star n In In1).
-          iFrame "∗ # %". }
-        exfalso. done. }
+      iApply (aacc_aupd_commit with "AU"); first done.
+      iIntros (C) "Hcss".
+      (* Now unfold CSS to execute unlockNode *)
+      iPoseProof (CSS_unfold_node with "[$] [$] [$] [$]")
+        as (I) "(Hn & HhIn & Hg & Hlock & Hns & Hcss')".
       iAaccIntro with "Hlock".
-      { iIntros "Hlock". iModIntro. iSplitR "Hfil Hb Hks".
-        iExists I. iFrame "∗ % #". iApply "Hstar". iExists true, In1.
-        iFrame "∗ # %". eauto with iFrame. }
-      iIntros "Hlock". iModIntro.
-      iPoseProof ((own_valid_2 (γ_h n) (●{1 / 2} In) (●{1 / 2} In1))
-                    with "[Hfil] [Hfis]") as "%"; try done.
-      apply (auth_auth_frac_op_inv _ _ _ _) in H2.
-      apply leibniz_equiv in H2. replace In1.
-      iSplitR "". iExists I.
-      iDestruct "Hb" as "(Hb & %)". subst Cn'.
-      iFrame "∗ % #". iApply "Hstar". iExists false, In. iFrame "∗ % #".
-      iExists Cn. iFrame. iIntros "AU". iModIntro. wp_pures.
-      iApply "IH"; try done.
+      { iIntros "Hlock". iModIntro.
+        iPoseProof ("Hcss'" with "[Hg Hlock Hns]") as "Hcss";
+          first eauto with iFrame.
+        iFrame "Hcss". iIntros "AU". iModIntro. iFrame "∗".
+      }
+      iIntros "Hlock". (* unlockNode finished executing *)
+      (* Linearization Point *)
+      iDestruct "Hg" as "(HI & Hglob & Hks & Hdom)".
+      iMod ((ghost_update_keyset γ_k dop k Cn Cn' res (keyset K In n) C)
+              with "[HkIn Hks]") as (C') "(#HΨC & Hks & HkIn)".
+      {
+        iPoseProof (keyset_valid with "HkIn") as "%".
+        assert (k ∈ keyset K In n); first by apply keyset_def.
+        iPoseProof ((Ψ_impl_C_in_K _ _ _ _ _ (keyset K In n))
+                      with "[$HΨ] [% //] [% //]") as "%".
+        iFrame "∗ #". by iPureIntro.
+      }
+      (* Close everything up, return *)
+      iModIntro. iExists C', res. iSpecialize ("Hcss'" $! C').
+      iPoseProof ("Hcss'" with "[-]") as "Hcss".
+      { iFrame "∗". iExists false, In. iFrame. iExists Cn'. iFrame "∗ #". }
+      iFrame "Hcss HΨC". iIntros "H". iModIntro. wp_pures. done.
+    - (* Case: decisiveOp fails *)
+      wp_pures. iDestruct "Hb" as "%". subst Cn'.
+      iAssert (nodePred γ_f γ_h γ_k n In Cn)%I
+        with "[$Hn $HnhIn $HkIn $Hinfp $domIn]" as "Hnp".
+      awp_apply (unlockNode_spec_high with "Hnp").
+      (* Open AU for unlockNode's pre *)
+      iApply (aacc_aupd_abort with "AU"); first done. iIntros (C) "Hcss".
+      iAaccIntro with "Hcss".
+      { iIntros. iModIntro. iFrame. iIntros "AU". iModIntro. iFrame. }
+      iIntros "Hcss". iModIntro.
+      (* Close up AU again *)
+      iFrame. iIntros "AU". iModIntro. 
+      wp_pures. by iApply "IH".
   Qed.
 
 End Link_Template.
+
