TODOs.md
@@ -1,6 +1,8 @@
 Things to do
 ------------
 
+- Why is Ψ iProp?
+
 - Can we prove the lock/unlock specs shown in the paper?
 
 - Why does traverse_spec return inFP(n') and domm In' = {[n']}?
@@ -22,3 +24,16 @@ Things to do
 - We can try to get rid of getLockLoc and just do CAS (lockLoc "l") #true #false in lock, etc.
 
 - Can we make `findNext` return a bool and a node instead of an option node to match implementations?
+
+
+Lessons learnt
+--------------
+
+- Use P -* Q -* R instead of P * Q -* R.
+
+- Avoid iFrame "∗ % #" its too slow.
+
+- Use `as (?C) "H"` pattern to introduce a fresh variable C0/C1/...
+
+- `iAssert (⌜False⌝)%I` can be replaced with `iExFalso`.
+
